src/PlutusIR/Semantics/SemanticEquivalence/Congruence.v
@@ -1,0 +1,14 @@
+Require Import Lists.List.
+From PlutusCert Require Import PlutusIR.
+From PlutusCert Require Import PlutusIR.Semantics.Static.Typing.
+
+Import ListNotations.
+
+(* congruence = equivalence relation + context_compatible *)
+Definition context_compatible R :=
+  forall Δ Γ s t T,
+    R Δ Γ s t T ->
+    forall (C : context) Δ1 Γ1 T1,
+      Δ1 ,, Γ1  |- C : (Δ, Γ, T) ↪ T1 ->
+        R Δ1 Γ1(context_fill C s) (context_fill C t) T1
+.
